Stop trying to keep track of boundaries in the syntax
instead, keep track of boundary states in the program logic

theories/interop/linking_wp.v
@@ -1,5 +1,6 @@
 From Coq Require Import ssreflect.
 From stdpp Require Import strings gmap.
+From iris.algebra.lib Require Import excl_auth.
 From melocoton.interop Require Import linking.
 From melocoton.mlanguage Require Import mlanguage.
 From melocoton.mlanguage Require Import weakestpre lifting.
@@ -7,11 +8,22 @@ From iris.proofmode Require Import proofmode.
 
 (* FIXME: the proofs in this file need cleanup *)
 
+Inductive link_state_case :=
+  Boundary | In1 | In2.
+
+Canonical Structure link_state_caseO := leibnizO link_state_case.
+
+Class linkG Σ := LinkG {
+  linkG_inG :> inG Σ (excl_authR (leibnizO link_state_case));
+  linkG_γ : gname;
+}.
+
 Section Linking_logic.
 Context {hlc : has_lc}.
 Context {Σ : gFunctors}.
 Context {val pubstate : Type}.
 Context (Λ1 Λ2 : mlanguage val pubstate).
+Context `{linkG Σ}.
 Context `{!publicStateInterp pubstate Σ}.
 Context `{!mlangGS hlc val pubstate Σ Λ1}.
 Context `{!mlangGS hlc val pubstate Σ Λ2}.
@@ -24,27 +36,92 @@ Implicit Types T : string -d> list val -d> (val -d> iPropO Σ) -d> iPropO Σ.
 Definition link_state_interp (st : (link_lang Λ1 Λ2).(state)) : iProp Σ :=
   match st with
   | LinkSt pubσ privσ1 privσ2 =>
+      own linkG_γ (●E Boundary) ∗
       public_state_interp pubσ ∗
       private_state_interp privσ1 ∗
       private_state_interp privσ2
   | LinkSt1 σ1 privσ2 =>
+      own linkG_γ (●E In1) ∗
       state_interp σ1 ∗ private_state_interp privσ2
   | LinkSt2 privσ1 σ2 =>
+      own linkG_γ (●E In2) ∗
       private_state_interp privσ1 ∗ state_interp σ2
   end.
+
+Definition link_state_frag case : iProp Σ :=
+  own linkG_γ (◯E case).
+
+Definition link_in_state case : iProp Σ :=
+  link_state_frag case ∗
+  match case with
+  | Boundary => at_boundary Λ1 ∗ at_boundary Λ2
+  | In1 => at_boundary Λ2
+  | In2 => at_boundary Λ1
+  end.
+
+Lemma link_state_update case case' :
+  own linkG_γ (●E case) -∗ link_state_frag case ==∗
+  own linkG_γ (●E case') ∗ link_state_frag case'.
+Proof using.
+  iIntros "Haa Haf". unfold link_state_frag.
+  iDestruct (own_op with "[$Haa $Haf]") as "H".
+  iMod (own_update with "H") as "H".
+  { eapply (excl_auth_update _ _ case'). }
+  by rewrite own_op.
+Qed.
+
+Lemma link_at_boundary st :
+  link_state_interp st ∗ link_state_frag Boundary -∗
+  ⌜∃ pubσ privσ1 privσ2, st = LinkSt pubσ privσ1 privσ2⌝.
+Proof using.
+  iIntros "[Hst Hb]". destruct st; eauto.
+  all: iDestruct "Hst" as "(Hb' & ?)".
+  all: iDestruct (own_op with "[$Hb' $Hb]") as "Hb".
+  all: iDestruct (own_valid with "Hb") as "%Hb".
+  all: by apply excl_auth_agree in Hb.
+Qed.
+
+Lemma link_at_in1 st :
+  link_state_interp st ∗ link_state_frag In1 -∗
+  ⌜∃ σ1 privσ2, st = LinkSt1 σ1 privσ2⌝.
+Proof using.
+  iIntros "[Hst Hb]". destruct st; eauto.
+  all: iDestruct "Hst" as "(Hb' & ?)".
+  all: iDestruct (own_op with "[$Hb' $Hb]") as "Hb".
+  all: iDestruct (own_valid with "Hb") as "%Hb".
+  all: by apply excl_auth_agree in Hb.
+Qed.
+
+Lemma link_at_in2 st :
+  link_state_interp st ∗ link_state_frag In2 -∗
+  ⌜∃ privσ1 σ2, st = LinkSt2 privσ1 σ2⌝.
+Proof using.
+  iIntros "[Hst Hb]". destruct st; eauto.
+  all: iDestruct "Hst" as "(Hb' & ?)".
+  all: iDestruct (own_op with "[$Hb' $Hb]") as "Hb".
+  all: iDestruct (own_valid with "Hb") as "%Hb".
+  all: by apply excl_auth_agree in Hb.
+Qed.
 
 Program Instance link_mlangGS : mlangGS hlc val pubstate Σ (link_lang Λ1 Λ2) := {
   state_interp := link_state_interp;
   private_state_interp := (λ '(privσ1, privσ2),
+    own linkG_γ (●E Boundary) ∗
     private_state_interp privσ1 ∗ private_state_interp privσ2)%I;
+  at_boundary := link_in_state Boundary;
 }.
 Next Obligation.
   simpl. iIntros (σ pubσ privσ). inversion 1; subst.
-  iIntros "(? & ? & ?)". by iFrame.
+  iIntros "(? & ? & ? & ?)". by iFrame.
 Qed.
 Next Obligation.
   simpl. iIntros (σ pubσ privσ). inversion 1; subst.
-  iIntros "(? & ? & ?)". by iFrame.
+  iIntros "(? & ? & ? & ?)". by iFrame.
+Qed.
+Next Obligation.
+  iIntros (σ) "((Hb & ? & ?) & Hσ)".
+  iDestruct (link_at_boundary with "[$Hb $Hσ]") as %(? & ? & ? & ->).
+  iPureIntro. eexists _, _. constructor.
 Qed.
 
 Lemma proj1_prog_union (pe1: mlanguage.prog Λ1) (pe2: mlanguage.prog Λ2) :
@@ -93,11 +170,15 @@ Class can_link_prog `{!invGS_gen hlc Σ}
   can_link_spec1 fname (func: mlanguage.func Λ2) vs Φ E :
     prog pe2 !! fname = Some func →
     T pe1 fname vs Φ -∗
-    ∃ e2, ⌜apply_func func vs = Some e2⌝ ∗ ▷ WP e2 @ pe2; E {{ Φ }};
+    ∃ e2, ⌜apply_func func vs = Some e2⌝ ∗ ▷
+      (at_boundary Λ2 -∗ WP e2 @ pe2; E {{
+        λ v, Φ v ∗ at_boundary Λ2 }});
   can_link_spec2 fname (func: mlanguage.func Λ1) vs Φ E :
     prog pe1 !! fname = Some func →
     T pe2 fname vs Φ -∗
-    ∃ e1, ⌜apply_func func vs = Some e1⌝ ∗ ▷ WP e1 @ pe1; E {{ Φ }};
+    ∃ e1, ⌜apply_func func vs = Some e1⌝ ∗ ▷
+      (at_boundary Λ1 -∗ WP e1 @ pe1; E {{
+        λ v, Φ v ∗ at_boundary Λ1 }});
 }.
 
 Lemma wp_link_call `{!invGS_gen hlc Σ}
@@ -112,8 +193,7 @@ Lemma wp_link_call `{!invGS_gen hlc Σ}
 Proof using.
   iIntros (pe Hfn) "Hwp".
   iApply (@wp_unfold _ _ _ _ _ _ (link_lang Λ1 Λ2)). rewrite /wp_pre.
-  iIntros (σ) "[Hσ %Hmatch]". iModIntro. iRight; iRight.
-  inversion Hmatch; subst.
+  iIntros (σ) "Hσ". iModIntro. iRight; iRight.
   iSplitR.
   { iPureIntro. eexists (λ _, True). eexists k, (LkE _ []). split; first done.
     eapply CallS; eauto. }
@@ -130,27 +210,32 @@ Lemma wp_link_run_function_1 `{!invGS_gen hlc Σ}
   let pe := link_environ pe1 pe2 in
   can_link_prog pe1 pe2 →
   prog pe1 !! fname = Some fn →
+  link_state_frag Boundary -∗
+  at_boundary Λ1 -∗
   T pe2 fname arg Ξ -∗
   (∀ e1, ⌜apply_func fn arg = Some e1⌝ -∗
-         WP e1 @ pe1; E {{ v, Ξ v }} -∗
+         WP e1 @ pe1; E {{ v, Ξ v ∗ at_boundary Λ1 }} -∗
+         link_state_frag In1 -∗
          WP LkE (LinkExpr1 Λ1 Λ2 e1) (inr k2 :: k) @ pe; E {{ Φ }}) -∗
   WP LkE (LinkRunFunction Λ1 Λ2 (inl fn) arg) (inr k2 :: k) @ pe; E {{ Φ }}.
 Proof using.
-  iIntros (pe Hcan_link Hfn) "HTΞ Hwp".
+  iIntros (pe Hcan_link Hfn) "Hb Hb1 HTΞ Hwp".
   iApply (@wp_unfold _ _ _ _ _ _ (link_lang Λ1 Λ2)). rewrite /wp_pre.
-  iIntros (σ) "[Hσ %Hmatch]". inversion Hmatch; subst.
+  iIntros (σ) "Hσ". iDestruct (link_at_boundary with "[$Hb $Hσ]") as %(pubσ&privσ1&privσ2&->).
   iRight; iRight.
   iPoseProof (can_link_spec2 _ _ _ _ E Hfn with "HTΞ") as (? Happlyfunc) "Hwpcall".
 
-  iDestruct "Hσ" as "(Hpubσ & Hprivσ1 & Hprivσ2)".
+  iDestruct "Hσ" as "(Hob & Hpubσ & Hprivσ1 & Hprivσ2)".
   iModIntro. iSplitR.
   { iPureIntro. exists (λ _, True). eexists _, (LkE _ []). split; [done|].
     destruct (merge_split_state pubσ privσ1) as [? ?]. eapply RunFunction1S; eauto. }
-  iIntros (X Hstep'). destruct Hstep' as (K' & [se1' k1'] & ? & Hstep'). simpl in *; simplify_eq.
+  iIntros (X Hstep'). destruct Hstep' as (K' & [se2' k2'] & ? & Hstep'). simpl in *; simplify_eq.
   inversion Hstep'; simplify_eq/=; []. iModIntro. iNext.
   iMod (@state_interp_join _ _ _ _ Λ1 with "[$Hprivσ1 $Hpubσ]") as "Hσ1". eassumption.
-  iModIntro. iExists _, _. iSplitR; first done. iFrame "Hprivσ2 Hσ1".
-  by iApply "Hwp".
+  iMod (link_state_update _ In1 with "Hob Hb") as "(Hob & Hb)".
+  iModIntro. iExists _, _. iSplitR; first done. iFrame.
+  iDestruct ("Hwpcall" with "Hb1") as "Hwpcall".
+  by iApply ("Hwp" with "[] Hwpcall Hb").
 Qed.
 
 Lemma wp_link_run_function_2 `{!invGS_gen hlc Σ}
@@ -161,27 +246,32 @@ Lemma wp_link_run_function_2 `{!invGS_gen hlc Σ}
   let pe := link_environ pe1 pe2 in
   can_link_prog pe1 pe2 →
   prog pe2 !! fname = Some fn →
+  link_state_frag Boundary -∗
+  at_boundary Λ2 -∗
   T pe1 fname arg Ξ -∗
   (∀ e2, ⌜apply_func fn arg = Some e2⌝ -∗
-         WP e2 @ pe2; E {{ v, Ξ v }} -∗
+         WP e2 @ pe2; E {{ v, Ξ v ∗ at_boundary Λ2 }} -∗
+         link_state_frag In2 -∗
          WP LkE (LinkExpr2 Λ1 Λ2 e2) (inl k1 :: k) @ pe; E {{ Φ }}) -∗
   WP LkE (LinkRunFunction Λ1 Λ2 (inr fn) arg) (inl k1 :: k) @ pe; E {{ Φ }}.
 Proof using.
-  iIntros (pe Hcan_link Hfn) "HTΞ Hwp".
+  iIntros (pe Hcan_link Hfn) "Hb Hb2 HTΞ Hwp".
   iApply (@wp_unfold _ _ _ _ _ _ (link_lang Λ1 Λ2)). rewrite /wp_pre.
-  iIntros (σ) "[Hσ %Hmatch]". inversion Hmatch; subst.
+  iIntros (σ) "Hσ". iDestruct (link_at_boundary with "[$Hb $Hσ]") as %(pubσ&privσ1&privσ2&->).
   iRight; iRight.
   iPoseProof (can_link_spec1 _ _ _ _ E Hfn with "HTΞ") as (? Happlyfunc) "Hwpcall".
 
-  iDestruct "Hσ" as "(Hpubσ & Hprivσ1 & Hprivσ2)".
+  iDestruct "Hσ" as "(Hob & Hpubσ & Hprivσ1 & Hprivσ2)".
   iModIntro. iSplitR.
   { iPureIntro. exists (λ _, True). eexists _, (LkE _ []). split; [done|].
     destruct (merge_split_state pubσ privσ2) as [? ?]. eapply RunFunction2S; eauto. }
   iIntros (X Hstep'). destruct Hstep' as (K' & [se2' k2'] & ? & Hstep'). simpl in *; simplify_eq.
   inversion Hstep'; simplify_eq/=; []. iModIntro. iNext.
   iMod (@state_interp_join _ _ _ _ Λ2 with "[$Hprivσ2 $Hpubσ]") as "Hσ2". eassumption.
-  iModIntro. iExists _, _. iSplitR; first done. iFrame "Hprivσ1 Hσ2".
-  by iApply "Hwp".
+  iMod (link_state_update _ In2 with "Hob Hb") as "(Hob & Hb)".
+  iModIntro. iExists _, _. iSplitR; first done. iFrame.
+  iDestruct ("Hwpcall" with "Hb2") as "Hwpcall".
+  by iApply ("Hwp" with "[] Hwpcall Hb").
 Qed.
 
 Lemma wp_link_retval_1 `{!invGS_gen hlc Σ}
@@ -190,13 +280,13 @@ Lemma wp_link_retval_1 `{!invGS_gen hlc Σ}
   E k1 v (Φ : val → iProp Σ)
 :
   let pe := link_environ pe1 pe2 in
-  WP LkSE (LinkExpr1 Λ1 Λ2 (fill k1 (of_val Λ1 v))) @ pe; E {{ Φ }} -∗
-  WP LkE (LinkExprV Λ1 Λ2 v) [inl k1] @ pe; E {{ Φ }}.
+  (link_state_frag In1 -∗ WP LkSE (LinkExpr1 Λ1 Λ2 (fill k1 (of_val Λ1 v))) @ pe; E {{ Φ }}) -∗
+  (link_state_frag Boundary -∗ WP LkE (LinkExprV Λ1 Λ2 v) [inl k1] @ pe; E {{ Φ }}).
 Proof using.
-  iIntros (pe) "Hwp".
+  iIntros (pe) "Hwp Hb".
   iApply (@wp_unfold _ _ _ _ _ _ (link_lang Λ1 Λ2)). rewrite /wp_pre.
-  iIntros (σ) "[Hσ %Hmatch']". inversion Hmatch'; subst. iModIntro. iRight. iRight.
-  iDestruct "Hσ" as "(Hpub & Hpriv1 & Hpriv2)".
+  iIntros (σ) "Hσ". iDestruct (link_at_boundary with "[$Hσ $Hb]") as %(pubσ&privσ1&privσ2&->).
+  iModIntro. iRight. iRight. iDestruct "Hσ" as "(Hob & Hpub & Hpriv1 & Hpriv2)".
   iSplitR.
   { iPureIntro. apply head_prim_reducible. exists (λ _, True).
     destruct (merge_split_state pubσ privσ1) as [? ?]. eapply Ret1S; eauto. }
@@ -204,8 +294,8 @@ Proof using.
   inversion Hstep'; simplify_eq/=; [].
   iModIntro. iNext.
   iMod (@state_interp_join _ _ _ _ Λ1 with "[$Hpriv1 $Hpub]") as "H1". eassumption.
-  iModIntro. iExists _, _. iSplitR; first done. iFrame "Hpriv2 H1".
-  by iFrame.
+  iMod (link_state_update _ In1 with "Hob Hb") as "(Hob & Hb)".
+  iModIntro. iExists _, _. iSplitR; first done. iFrame. iApply "Hwp". iFrame.
 Qed.
 
 Lemma wp_link_retval_2 `{!invGS_gen hlc Σ}
@@ -214,13 +304,13 @@ Lemma wp_link_retval_2 `{!invGS_gen hlc Σ}
   E k2 v (Φ : val → iProp Σ)
 :
   let pe := link_environ pe1 pe2 in
-  WP LkSE (LinkExpr2 Λ1 Λ2 (fill k2 (of_val Λ2 v))) @ pe; E {{ Φ }} -∗
-  WP LkE (LinkExprV Λ1 Λ2 v) [inr k2] @ pe; E {{ Φ }}.
+  (link_state_frag In2 -∗ WP LkSE (LinkExpr2 Λ1 Λ2 (fill k2 (of_val Λ2 v))) @ pe; E {{ Φ }}) -∗
+  (link_state_frag Boundary -∗ WP LkE (LinkExprV Λ1 Λ2 v) [inr k2] @ pe; E {{ Φ }}).
 Proof using.
-  iIntros (pe) "Hwp".
+  iIntros (pe) "Hwp Hb".
   iApply (@wp_unfold _ _ _ _ _ _ (link_lang Λ1 Λ2)). rewrite /wp_pre.
-  iIntros (σ) "[Hσ %Hmatch']". inversion Hmatch'; subst. iModIntro. iRight. iRight.
-  iDestruct "Hσ" as "(Hpub & Hpriv1 & Hpriv2)".
+  iIntros (σ) "Hσ". iDestruct (link_at_boundary with "[$Hσ $Hb]") as %(pubσ&privσ1&privσ2&->).
+  iModIntro. iRight. iRight. iDestruct "Hσ" as "(Hob & Hpub & Hpriv1 & Hpriv2)".
   iSplitR.
   { iPureIntro. apply head_prim_reducible. eexists (λ _, True).
     destruct (merge_split_state pubσ privσ2). eapply Ret2S; eauto. }
@@ -228,8 +318,8 @@ Proof using.
   inversion Hstep'; simplify_eq/=; [].
   iModIntro. iNext.
   iMod (@state_interp_join _ _ _ _ Λ2 with "[$Hpriv2 $Hpub]") as "H2". eassumption.
-  iModIntro. iExists _, _. iSplitR; first done. iFrame "Hpriv1 H2".
-  by iFrame.
+  iMod (link_state_update _ In2 with "Hob Hb") as "(Hob & Hb)".
+  iModIntro. iExists _, _. iSplitR; first done. iFrame. iApply "Hwp". iFrame.
 Qed.
 
 Lemma wp_link_extcall_1 `{!invGS_gen hlc Σ}
@@ -241,21 +331,27 @@ Lemma wp_link_extcall_1 `{!invGS_gen hlc Σ}
   prog pe1 !! fn_name = None →
   prog pe2 !! fn_name = None →
   T pe1 fn_name arg Ξ -∗
-  (▷ ∀ r : val, Ξ r -∗ WP fill (comp_ectx k1 empty_ectx) (of_class Λ1 (ExprVal r)) @ pe1; E {{ Φ }}) -∗
-  (▷ ∀ r, WP fill k1 (of_class Λ1 (ExprVal r)) @ pe1; E {{ Φ }} -∗
-        WP LkE (LinkExprV Λ1 Λ2 r) [inl k1] @ pe; E {{ Φ }}) -∗
-  WP LkE (LinkExprCall Λ1 Λ2 fn_name arg) [inl k1] @ pe; E {{ Φ }}.
+  (▷ ∀ r : val, Ξ r ∗ at_boundary Λ1 -∗
+        WP fill (comp_ectx k1 empty_ectx) (of_class Λ1 (ExprVal r)) @ pe1; E {{ λ v, Φ v ∗ at_boundary Λ1 }}) -∗
+  (▷ ∀ r, WP fill k1 (of_class Λ1 (ExprVal r)) @ pe1; E {{ λ v, Φ v ∗ at_boundary Λ1 }} -∗
+        link_state_frag Boundary -∗
+        at_boundary Λ2 -∗
+        WP LkE (LinkExprV Λ1 Λ2 r) [inl k1] @ pe; E {{ λ v, Φ v ∗ at_boundary (link_lang Λ1 Λ2) }}) -∗
+  at_boundary (link_lang Λ1 Λ2) -∗
+  WP LkE (LinkExprCall Λ1 Λ2 fn_name arg) [inl k1] @ pe; E {{ λ v, Φ v ∗ at_boundary (link_lang Λ1 Λ2) }}.
 Proof using.
-  iIntros (pe Hfn1 Hfn2) "HTΞ HΞ Hwp".
+  iIntros (pe Hfn1 Hfn2) "HTΞ HΞ Hwp (Hb & Hb1 & Hb2)".
   assert (Hpef: prog pe !! fn_name = None).
   { apply lookup_union_None. rewrite !lookup_fmap Hfn1 Hfn2 //. }
   iApply (@wp_unfold _ _ _ _ _ _ (link_lang Λ1 Λ2)). rewrite /wp_pre.
-  iIntros (σ) "[Hσ %Hmatch']". inversion Hmatch'; subst.
+  iIntros (σ) "Hσ". iDestruct (link_at_boundary with "[$Hσ $Hb]") as %(pubσ&privσ1&privσ2&->).
   iModIntro. iRight; iLeft. iExists _, _, [inl k1]. iSplitR; [by eauto|].
-  iSplitR; first by eauto. iModIntro. iFrame "Hσ". iExists Ξ. iSplitL "HTΞ".
+  iSplitR; first by eauto. iFrame "Hσ Hb Hb1 Hb2". iExists Ξ. iSplitL "HTΞ".
   { rewrite /pe /=. iSplitR; [now iPureIntro; split; eauto|]. iLeft. iApply "HTΞ". }
-  iNext. iIntros (r) "Hr". simpl. iSpecialize ("HΞ" with "Hr"). rewrite -fill_comp fill_empty.
-  by iApply "Hwp".
+  iNext. iIntros (r) "[Hr Hb]". iDestruct "Hb" as "(Hb & Hb1 & Hb2)".
+  simpl.
+  iSpecialize ("HΞ" with "[$Hr $Hb1]"). rewrite -fill_comp fill_empty.
+  iApply ("Hwp" with "HΞ Hb Hb2").
 Qed.
 
 Lemma wp_link_extcall_2 `{!invGS_gen hlc Σ}
@@ -267,22 +363,27 @@ Lemma wp_link_extcall_2 `{!invGS_gen hlc Σ}
   prog pe1 !! fn_name = None →
   prog pe2 !! fn_name = None →
   T pe2 fn_name arg Ξ -∗
-  (▷ ∀ r : val, Ξ r -∗ WP fill (comp_ectx k2 empty_ectx) (of_class Λ2 (ExprVal r)) @ pe2; E {{ Φ }}) -∗
-  (▷ ∀ r, WP fill k2 (of_class Λ2 (ExprVal r)) @ pe2; E {{ Φ }} -∗
-        WP LkE (LinkExprV Λ1 Λ2 r) [inr k2] @ pe; E {{ Φ }}) -∗
-  WP LkE (LinkExprCall Λ1 Λ2 fn_name arg) [inr k2] @ pe; E {{ Φ }}.
+  (▷ ∀ r : val, Ξ r ∗ at_boundary Λ2 -∗
+        WP fill (comp_ectx k2 empty_ectx) (of_class Λ2 (ExprVal r)) @ pe2; E {{ λ v, Φ v ∗ at_boundary Λ2 }}) -∗
+  (▷ ∀ r, WP fill k2 (of_class Λ2 (ExprVal r)) @ pe2; E {{ λ v, Φ v ∗ at_boundary Λ2 }} -∗
+        link_state_frag Boundary -∗
+        at_boundary Λ1 -∗
+        WP LkE (LinkExprV Λ1 Λ2 r) [inr k2] @ pe; E {{ λ v, Φ v ∗ at_boundary (link_lang Λ1 Λ2) }}) -∗
+  at_boundary (link_lang Λ1 Λ2) -∗
+  WP LkE (LinkExprCall Λ1 Λ2 fn_name arg) [inr k2] @ pe; E {{ λ v, Φ v ∗ at_boundary (link_lang Λ1 Λ2) }}.
 Proof using.
-  iIntros (pe Hfn1 Hfn2) "HTΞ HΞ Hwp".
+  iIntros (pe Hfn1 Hfn2) "HTΞ HΞ Hwp (Hb & Hb1 & Hb2)".
   assert (Hpef: prog pe !! fn_name = None).
   { apply lookup_union_None. rewrite !lookup_fmap Hfn1 Hfn2 //. }
   iApply (@wp_unfold _ _ _ _ _ _ (link_lang Λ1 Λ2)). rewrite /wp_pre.
-  iIntros (σ) "[Hσ %Hmatch']". inversion Hmatch'; subst.
+  iIntros (σ) "Hσ". iDestruct (link_at_boundary with "[$Hσ $Hb]") as %(pubσ&privσ1&privσ2&->).
   iModIntro. iRight; iLeft. iExists _, _, [inr k2]. iSplitR; [by eauto|].
-  iSplitR; first by eauto.
-  iModIntro. iFrame "Hσ". iExists Ξ. iSplitL "HTΞ".
+  iSplitR; first by eauto. iFrame "Hσ Hb Hb1 Hb2". iExists Ξ. iSplitL "HTΞ".
   { rewrite /pe /=. iSplitR; [now iPureIntro; split; eauto|]. iRight. iApply "HTΞ". }
-  iNext. iIntros (r) "Hr". simpl. iSpecialize ("HΞ" with "Hr"). rewrite -fill_comp fill_empty.
-  by iApply "Hwp".
+  iNext. iIntros (r) "[Hr Hb]". iDestruct "Hb" as "(Hb & Hb1 & Hb2)".
+  simpl.
+  iSpecialize ("HΞ" with "[$Hr $Hb2]"). rewrite -fill_comp fill_empty.
+  iApply ("Hwp" with "HΞ Hb Hb1").
 Qed.
 
 Lemma link_head_step_call_ext_1_inv `{!invGS_gen hlc Σ} pe1 pe2 K f vs σ1 privσ2 X :
@@ -302,7 +403,9 @@ Proof using.
     rewrite proj1_prog_union in HH; [| apply Hcan_link]. congruence. }
   { exfalso. match goal with H:_|-_ => apply mk_is_Some in H; apply fill_val in H; destruct H as [? HH] end.
     rewrite /to_val to_of_class // in HH. }
-  rename H into Hfill. rename H3 into Hnofn. rewrite proj1_prog_union in Hnofn;[|apply Hcan_link].
+  match goal with H: fill _ _ = fill _ _ |- _ => rename H into Hfill end.
+  match goal with H: proj1_prog _ _ _ !! _ = None |- _ => rename H into Hnofn end.
+  rewrite proj1_prog_union in Hnofn;[|apply Hcan_link].
   pose proof (call_in_ctx_to_val _ _ _ _ _ Hfill) as [[K'' ->]|Hval].
   2: { exfalso. unfold to_val in Hval. destruct Hval. by repeat case_match. }
   rewrite -fill_comp in Hfill. apply fill_inj in Hfill. subst e1.
@@ -310,7 +413,8 @@ Proof using.
   destruct HH as [->|[? HH]].
   2: { exfalso. rewrite to_of_class in HH. congruence. }
   do 3 eexists; repeat split; eauto.
-  rewrite fill_empty to_of_class in H2. by simplify_eq/=.
+  match goal with H: to_class _ = Some _ |- _ => rename H into Hcall end.
+  rewrite fill_empty to_of_class in Hcall. by simplify_eq/=.
 Qed.
 
 Lemma link_head_step_call_ext_2_inv `{!invGS_gen hlc Σ} pe1 pe2 K f vs σ2 privσ1 X :
@@ -329,7 +433,9 @@ Proof using.
     rewrite proj2_prog_union in HH; [| apply Hcan_link]. congruence. }
   { exfalso. match goal with H:_|-_ => apply mk_is_Some in H; apply fill_val in H; destruct H as [? HH] end.
     rewrite /to_val to_of_class // in HH. }
-  rename H into Hfill. rename H3 into Hnofn. rewrite proj2_prog_union in Hnofn;[|apply Hcan_link].
+  match goal with H: fill _ _ = fill _ _ |- _ => rename H into Hfill end.
+  match goal with H: proj2_prog _ _ _ !! _ = None |- _ => rename H into Hnofn end.
+  rewrite proj2_prog_union in Hnofn;[|apply Hcan_link].
   pose proof (call_in_ctx_to_val _ _ _ _ _ Hfill) as [[K'' ->]|Hval].
   2: { exfalso. unfold to_val in Hval. destruct Hval. by repeat case_match. }
   rewrite -fill_comp in Hfill. apply fill_inj in Hfill. subst e2.
@@ -337,7 +443,8 @@ Proof using.
   destruct HH as [->|[? HH]].
   2: { exfalso. rewrite to_of_class in HH. congruence. }
   do 3 eexists; repeat split; eauto.
-  rewrite fill_empty to_of_class in H2. by simplify_eq/=.
+  match goal with H: to_class _ = Some _ |- _ => rename H into Hcall end.
+  rewrite fill_empty to_of_class in Hcall. by simplify_eq/=.
 Qed.
 
 Lemma wp_link_run `{!invGS_gen hlc Σ}
@@ -348,55 +455,59 @@ Lemma wp_link_run `{!invGS_gen hlc Σ}
   let pe := link_environ pe1 pe2 in
   can_link_prog pe1 pe2 →
   ⊢ □ (
-    (∀ e1 Φ, WP e1 @ pe1; E {{ Φ }} -∗
-             WP (LkSE (LinkExpr1 Λ1 Λ2 e1)) @ pe; E {{ Φ }}) ∗
-    (∀ e2 Φ, WP e2 @ pe2; E {{ Φ }} -∗
-             WP (LkSE (LinkExpr2 Λ1 Λ2 e2)) @ pe; E {{ Φ }})
+    (∀ e1 Φ, WP e1 @ pe1; E {{ λ v, Φ v ∗ at_boundary Λ1 }} -∗ link_in_state In1 -∗
+             WP (LkSE (LinkExpr1 Λ1 Λ2 e1)) @ pe; E {{ λ v, Φ v ∗ link_in_state Boundary }}) ∗
+    (∀ e2 Φ, WP e2 @ pe2; E {{ λ v, Φ v ∗ at_boundary Λ2 }} -∗ link_in_state In2 -∗
+             WP (LkSE (LinkExpr2 Λ1 Λ2 e2)) @ pe; E {{ λ v, Φ v ∗ link_in_state Boundary }})
   ).
 Proof using.
   intros pe Hcan_link. iLöb as "IH". iModIntro. iSplitL.
   (* Case 1: running Λ1 *)
-  { iIntros (e1 Φ) "Hwp".
+  { iIntros (e1 Φ) "Hwp [Hb Hb2]".
     rewrite wp_unfold. rewrite /wp_pre.
     iApply (@wp_unfold _ _ _ _ _ _ (link_lang Λ1 Λ2)). rewrite /wp_pre.
-    iIntros (σ) "[Hσ %Hmatch]".
-    inversion Hmatch; subst. iDestruct "Hσ" as "(Hσ1 & Hpriv2)".
-    iMod ("Hwp" $! σ1 with "[$Hσ1]") as "[Hwp|[Hwp|Hwp]]"; first done.
+    iIntros (σ) "Hσ". iDestruct (link_at_in1 with "[$Hb $Hσ]") as %(σ1 & privσ2 & ->).
+    iDestruct "Hσ" as "(Hob & Hσ1 & Hpriv2)".
+    iMod ("Hwp" $! σ1 with "[$Hσ1]") as "[Hwp|[Hwp|Hwp]]".
 
     (* WP: value case *)
-    { iDestruct "Hwp" as (v ->) "[Hσ HΦ]". iModIntro. iRight; iRight.
+    { iDestruct "Hwp" as (v ->) "[Hσ [HΦ Hb1]]".
+      iModIntro. iRight; iRight.
       (* administrative step Val1S: LinkExpr1 ~> LinkExprV *)
+      iDestruct (@splittable_at_boundary with "[$Hb1 $Hσ]") as %(pubσ&privσ1&Hsplitσ1).
       assert (Hhred: head_reducible (prog pe) (LkSE (LinkExpr1 Λ1 Λ2 (of_class Λ1 (ExprVal v)))) (LinkSt1 σ1 privσ2)).
-      { destruct (val_matching_split _ _ ltac:(eassumption)) as (pubσ&privσ1&Hsplitσ1).
-        exists (λ _, True). eapply Val1S; eauto. rewrite /to_val to_of_class //=. }
+      { exists (λ _, True). eapply Val1S; eauto. rewrite /to_val to_of_class //=. }
       iSplitR; [iPureIntro; by apply head_prim_reducible|].
       iIntros (X Hstep). apply head_reducible_prim_step in Hstep; [|done].
       inversion Hstep; simplify_eq/=.
       { exfalso. by match goal with H:_ |- _ => apply val_prim_step in H end. }
       { rewrite /to_val to_of_class in H3; simplify_eq/=.
         iMod (@state_interp_split _ _ _ _ Λ1 with "Hσ") as "[Hpriv1 Hpub]"; first by eauto.
-        iExists _, _. iSplitR; first done. iFrame. do 3 iModIntro.
-        by iApply wp_value. }
+        iExists _, _. iSplitR; first done.
+        iMod (link_state_update _ Boundary with "Hob Hb") as "[Hob Hb]".
+        do 3 iModIntro. iFrame. by iApply wp_value. }
       { exfalso.
         assert (is_Some (to_val e1)) as [? ?].
-        { eapply fill_val. eexists. unfold to_val. erewrite H. rewrite to_of_class//. }
-        unfold to_val in H0. repeat case_match; congruence. } }
+        { eapply fill_val. eexists. unfold to_val. erewrite H0. rewrite to_of_class//. }
+        unfold to_val in H1. repeat case_match; congruence. } }
 
     (* WP: call case *)
-    { iDestruct "Hwp" as (f vs K -> Hf) "Hcall". iModIntro. iRight; iRight.
+    { iDestruct "Hwp" as (f vs K -> Hf) "(Hb1 & Hσ1 & Hcall)". iModIntro. iRight; iRight.
       (* administrative step MakeCall1S: LinkExpr1 ~> LinkExprCall *)
+      iDestruct (@splittable_at_boundary with "[$Hb1 $Hσ1]") as %(pubσ&privσ1&Hsplitσ1).
       assert (head_reducible (prog pe) (LkSE (LinkExpr1 Λ1 Λ2 (fill K (of_class Λ1 (ExprCall f vs))))) (LinkSt1 σ1 privσ2)).
-      { apply matching_expr_state_ctx in H2.
-        destruct (call_matching_split _ _ _ ltac:(eassumption)) as (?&?&?).
-        exists (λ _, True). eapply MakeCall1S; eauto. by rewrite to_of_class.
+      { exists (λ _, True). eapply MakeCall1S; eauto. by rewrite to_of_class.
         rewrite proj1_prog_union; [done | apply Hcan_link]. }
       iSplitR; [iPureIntro; by apply head_prim_reducible|].
       iIntros (X Hstep). apply head_reducible_prim_step in Hstep;[|done].
+      clear pubσ privσ1 Hsplitσ1.
       eapply link_head_step_call_ext_1_inv in Hstep as (pubσ&privσ1&k1&->&?&?); eauto.
 
-      iMod "Hcall" as "[Hσ Hcall]". iDestruct "Hcall" as (Ξ) "[HTΞ HΞ]".
-      iMod (@state_interp_split _ _ _ _ Λ1 with "Hσ") as "[Hpriv1 Hpub]"; eauto.
-      iModIntro. iNext. iModIntro. iExists _, _. iSplitR; first done. iFrame.
+      iDestruct "Hcall" as (Ξ) "[HTΞ HΞ]".
+      iMod (@state_interp_split _ _ _ _ Λ1 with "Hσ1") as "[Hpriv1 Hpub]"; first done.
+      iMod (link_state_update _ Boundary with "Hob Hb") as "[Hob Hb]".
+      do 3 iModIntro. iExists _, _. iSplitR; first done. simpl.
+      iFrame "Hob Hpub Hpriv1 Hpriv2".
 
       (* two cases: this is an external call of the linking module itself, or it
          is a call to a function of pe2 *)
@@ -409,27 +520,31 @@ Proof using.
         (* administrative step CallS: LinkExprCall ~> LinkRunFunction *)
         iApply wp_link_call; first done.
         (* administrative step RunFunction2S: LinkRunFunction ~> LinkExpr2 *)
-        iApply (wp_link_run_function_2 with "HTΞ"); first done. iIntros (e2 He2) "Hwpcall".
+        iApply (wp_link_run_function_2 with "Hb Hb2 HTΞ"); first done.
+        iIntros (e2 He2) "Hwpcall Hb".
 
         progress change (LkE (LinkExpr2 Λ1 Λ2 e2) [inl k1]) with
           (linking.fill _ _ ([inl k1]:ectx (link_lang Λ1 Λ2)) (LkSE (LinkExpr2 Λ1 Λ2 e2))).
         iApply (@wp_bind _ _ _ _ _ _ (link_lang Λ1 Λ2)).
-        iApply ((@wp_wand _ _ _ _ _ _ (link_lang Λ1 Λ2)) with "[Hwpcall]").
-        { iDestruct "IH" as "#[_ IH2]". iApply "IH2". iApply "Hwpcall". }
-        iIntros (r) "Hr". iSpecialize ("HΞ" with "Hr"). rewrite -fill_comp fill_empty. simpl.
+        iApply ((@wp_wand _ _ _ _ _ _ (link_lang Λ1 Λ2)) with "[Hwpcall Hb Hb1]").
+        { iDestruct "IH" as "#[_ IH2]". iApply ("IH2" with "Hwpcall [$Hb $Hb1]"). }
+        iIntros (r) "[Hr (Hb & Hb1 & Hb2)]". iSpecialize ("HΞ" $! r).
+        rewrite -fill_comp fill_empty. simpl.
 
         (* administrative step Ret1S: LinkExprV ~> LinkExpr1 *)
-        iApply wp_link_retval_1.
+        iApply (wp_link_retval_1 with "[-Hb] Hb"). iIntros "Hb".
         (* continue the execution by induction *)
-        iDestruct "IH" as "#[IH1 _]". iApply "IH1". unfold of_val. done. }
+        iDestruct "IH" as "#[IH1 _]". iApply ("IH1" with "[-Hb Hb2] [$Hb $Hb2]"). unfold of_val.
+        iApply "HΞ". iFrame. }
 
       { (* external call *)
-        iApply (wp_link_extcall_1 with "HTΞ HΞ"); auto. iNext.
-        iIntros (r) "HΞ".
+        iApply (wp_link_extcall_1 with "HTΞ HΞ [] [$Hb $Hb1 $Hb2]"); auto.
+        iNext.
+        iIntros (r) "HΞ Hb Hb2".
         (* administrative step Ret1S: LinkExprV ~> LinkExpr1 *)
-        iApply wp_link_retval_1.
+        iApply (wp_link_retval_1 with "[-Hb] Hb"). iIntros "Hb".
         (* continue the execution by induction *)
-        iDestruct "IH" as "#[IH1 _]". iApply "IH1". unfold of_val. done. } }
+        iDestruct "IH" as "#[IH1 _]". iApply ("IH1" with "HΞ [$Hb $Hb2]"). } }
 
     { (* WP: step case *)
       iDestruct "Hwp" as (Hred) "Hwp". iModIntro. iRight; iRight.
@@ -443,55 +558,58 @@ Proof using.
         clear Hstep. rename H5 into Hstep.
         rewrite proj1_prog_union in Hstep; [|apply Hcan_link].
         iSpecialize ("Hwp" $! _ Hstep). iMod "Hwp". iIntros "!>!>". iMod "Hwp" as (e' σ' HX) "[Hσ Hwp]".
-        iModIntro. iExists _, _. iSplitR; [iPureIntro; naive_solver|]. iFrame.
-        iDestruct "IH" as "[IH1 _]". iApply ("IH1" with "Hwp"). }
+        iModIntro. iExists _, _. iSplitR; [iPureIntro; naive_solver|]. iFrame "Hσ Hob Hpriv2".
+        iDestruct "IH" as "[IH1 _]". iApply ("IH1" with "Hwp [$Hb $Hb2]"). }
       { exfalso. apply reducible_not_val in Hred. congruence. }
       { exfalso. clear Hstep. erewrite <-(of_to_class e0) in Hred; [|eassumption].
         rewrite proj1_prog_union in H5;[|apply Hcan_link].
         destruct Hred as (?&Hred). eapply extcall_ctx_irreducible; eauto. } } }
 
   (* Case 2: running Λ2 *)
-  { iIntros (e2 Φ) "Hwp".
+  { iIntros (e2 Φ) "Hwp [Hb Hb1]".
     rewrite wp_unfold. rewrite /wp_pre.
     iApply (@wp_unfold _ _ _ _ _ _ (link_lang Λ1 Λ2)). rewrite /wp_pre.
-    iIntros (σ) "[Hσ %Hmatch]".
-    inversion Hmatch; subst. iDestruct "Hσ" as "(Hprivσ1 & Hσ2)".
-    iMod ("Hwp" $! σ2 with "[$Hσ2]") as "[Hwp|[Hwp|Hwp]]"; first done.
+    iIntros (σ) "Hσ". iDestruct (link_at_in2 with "[$Hb $Hσ]") as %(privσ1 & σ2 & ->).
+    iDestruct "Hσ" as "(Hob & Hpriv1 & Hσ2)".
+    iMod ("Hwp" $! σ2 with "[$Hσ2]") as "[Hwp|[Hwp|Hwp]]".
 
     (* WP: value case *)
-    { iDestruct "Hwp" as (v ->) "[Hσ HΦ]". iModIntro. iRight; iRight.
+    { iDestruct "Hwp" as (v ->) "[Hσ [HΦ Hb2]]". iModIntro. iRight; iRight.
       (* administrative step Val2S: LinkExpr2 ~> LinkExprV *)
+      iDestruct (@splittable_at_boundary with "[$Hb2 $Hσ]") as %(pubσ&privσ2&Hsplitσ2).
       assert (Hhred: head_reducible (prog pe) (LkSE (LinkExpr2 Λ1 Λ2 (of_class Λ2 (ExprVal v)))) (LinkSt2 privσ1 σ2)).
-      { destruct (val_matching_split _ _ ltac:(eassumption)) as (?&?&?).
-        exists (λ _, True). eapply Val2S; eauto. rewrite /to_val to_of_class //=. }
+      { exists (λ _, True). eapply Val2S; eauto. rewrite /to_val to_of_class //=. }
       iSplitR; [iPureIntro; by apply head_prim_reducible|].
       iIntros (X Hstep). apply head_reducible_prim_step in Hstep; [|done].
       inversion Hstep; simplify_eq/=.
       { exfalso. by match goal with H:_ |- _ => apply val_prim_step in H end. }
       { rewrite /to_val to_of_class in H3; simplify_eq/=.
         iMod (@state_interp_split _ _ _ _ Λ2 with "Hσ") as "[Hpriv2 Hpub]"; first by eauto.
-        iExists _, _. iSplitR; first done. iFrame. iModIntro. iNext. iModIntro.
-        by iApply wp_value. }
+        iExists _, _. iSplitR; first done.
+        iMod (link_state_update _ Boundary with "Hob Hb") as "[Hob Hb]".
+        do 3 iModIntro. iFrame. by iApply wp_value. }
       { exfalso.
         assert (is_Some (to_val e2)) as [? ?].
-        { eapply fill_val. eexists. unfold to_val. erewrite H. rewrite to_of_class//. }
-        unfold to_val in H0. repeat case_match; congruence. } }
+        { eapply fill_val. eexists. unfold to_val. erewrite H0. rewrite to_of_class//. }
+        unfold to_val in H1. repeat case_match; congruence. } }
 
     (* WP: call case *)
-    { iDestruct "Hwp" as (f vs K -> Hf) "Hcall". iModIntro. iRight; iRight.
+    { iDestruct "Hwp" as (f vs K -> Hf) "(Hb2 & Hσ2 & Hcall)". iModIntro. iRight; iRight.
       (* administrative step MakeCall1S: LinkExpr2 ~> LinkExprCall *)
+      iDestruct (@splittable_at_boundary with "[$Hb2 $Hσ2]") as %(pubσ&privσ2&Hsplitσ2).
       assert (head_reducible (prog pe) (LkSE (LinkExpr2 Λ1 Λ2 (fill K (of_class Λ2 (ExprCall f vs))))) (LinkSt2 privσ1 σ2)).
-      { apply matching_expr_state_ctx in H2.
-        destruct (call_matching_split _ _ _ ltac:(eassumption)) as (?&?&?).
-        exists (λ _, True). eapply MakeCall2S; eauto. by rewrite to_of_class.
+      { exists (λ _, True). eapply MakeCall2S; eauto. by rewrite to_of_class.
         rewrite proj2_prog_union; [done | apply Hcan_link]. }
       iSplitR; [iPureIntro; by apply head_prim_reducible|].
       iIntros (X Hstep). apply head_reducible_prim_step in Hstep;[|done].
+      clear pubσ privσ2 Hsplitσ2.
       eapply link_head_step_call_ext_2_inv in Hstep as (pubσ&privσ2&k2&->&?&?); eauto.
 
-      iMod "Hcall" as "[Hσ Hcall]". iDestruct "Hcall" as (Ξ) "[HTΞ HΞ]".
-      iMod (@state_interp_split _ _ _ _ Λ2 with "Hσ") as "[Hpub Hpriv2]"; eauto.
-      iModIntro. iNext. iModIntro. iExists _, _. iSplitR; first done. iFrame.
+      iDestruct "Hcall" as (Ξ) "[HTΞ HΞ]".
+      iMod (@state_interp_split _ _ _ _ Λ2 with "Hσ2") as "[Hpub Hpriv2]"; first done.
+      iMod (link_state_update _ Boundary with "Hob Hb") as "[Hob Hb]".
+      do 3 iModIntro. iExists _, _. iSplitR; first done. simpl.
+      iFrame "Hob Hpub Hpriv1 Hpriv2".
 
       (* two cases: this is an external call of the linking module itself, or it
          is a call to a function of pe2 *)
@@ -504,27 +622,30 @@ Proof using.
         (* administrative step CallS: LinkExprCall ~> LinkRunFunction *)
         iApply wp_link_call; first done.
         (* administrative step RunFunction1S: LinkRunFunction ~> LinkExpr1 *)
-        iApply (wp_link_run_function_1 with "HTΞ"); first done. iIntros (e1 He1) "Hwpcall".
+        iApply (wp_link_run_function_1 with "Hb Hb1 HTΞ"); first done.
+        iIntros (e1 He1) "Hwpcall Hb".
 
         progress change (LkE (LinkExpr1 Λ1 Λ2 e1) [inr k2]) with
           (linking.fill _ _ ([inr k2]:ectx (link_lang Λ1 Λ2)) (LkSE (LinkExpr1 Λ1 Λ2 e1))).
         iApply (@wp_bind _ _ _ _ _ _ (link_lang Λ1 Λ2)).
-        iApply ((@wp_wand _ _ _ _ _ _ (link_lang Λ1 Λ2)) with "[Hwpcall]").
-        { iDestruct "IH" as "#[IH1 _]". iApply "IH1". iApply "Hwpcall". }
-        iIntros (r) "Hr". iSpecialize ("HΞ" with "Hr"). rewrite -fill_comp fill_empty. simpl.
+        iApply ((@wp_wand _ _ _ _ _ _ (link_lang Λ1 Λ2)) with "[Hwpcall Hb Hb2]").
+        { iDestruct "IH" as "#[IH1 _]". iApply ("IH1" with "Hwpcall [$Hb $Hb2]"). }
+        iIntros (r) "[Hr (Hb & Hb1 & Hb2)]". iSpecialize ("HΞ" $! r).
+        rewrite -fill_comp fill_empty. simpl.
 
         (* administrative step Ret2S: LinkExprV ~> LinkExpr2 *)
-        iApply wp_link_retval_2.
+        iApply (wp_link_retval_2 with "[-Hb] Hb"). iIntros "Hb".
         (* continue the execution by induction *)
-        iDestruct "IH" as "#[_ IH2]". iApply "IH2". unfold of_val. done. }
+        iDestruct "IH" as "#[_ IH2]". iApply ("IH2" with "[-Hb Hb1] [$Hb $Hb1]"). unfold of_val.
+        iApply "HΞ". iFrame. }
 
       { (* external call *)
-        iApply (wp_link_extcall_2 with "HTΞ HΞ"); auto. iNext.
-        iIntros (r) "HΞ".
+        iApply (wp_link_extcall_2 with "HTΞ HΞ [] [$Hb $Hb1 $Hb2]"); auto. iNext.
+        iIntros (r) "HΞ Hb Hb1".
         (* administrative step Ret1S: LinkExprV ~> LinkExpr1 *)
-        iApply wp_link_retval_2.
+        iApply (wp_link_retval_2 with "[-Hb] Hb"). iIntros "Hb".
         (* continue the execution by induction *)
-        iDestruct "IH" as "#[_ IH2]". iApply "IH2". unfold of_val. done. } }
+        iDestruct "IH" as "#[_ IH2]". iApply ("IH2" with "HΞ [$Hb $Hb1]"). } }
 
     { (* WP: step case *)
       iDestruct "Hwp" as (Hred) "Hwp". iModIntro. iRight; iRight.
@@ -539,8 +660,8 @@ Proof using.
         clear Hstep. rename H5 into Hstep.
         rewrite proj2_prog_union in Hstep; [|apply Hcan_link].
         iSpecialize ("Hwp" $! _ Hstep). iMod "Hwp". iIntros "!>!>". iMod "Hwp" as (e' σ' HX) "[Hσ Hwp]".
-        iModIntro. iExists _, _. iSplitR; [iPureIntro; naive_solver|]. iFrame.
-        iDestruct "IH" as "[_ IH2]". iApply ("IH2" with "Hwp"). }
+        iModIntro. iExists _, _. iSplitR; [iPureIntro; naive_solver|]. iFrame "Hob Hσ Hpriv1".
+        iDestruct "IH" as "[_ IH2]". iApply ("IH2" with "Hwp [$Hb $Hb1]"). }
       { exfalso. apply reducible_not_val in Hred. congruence. }
       { exfalso. clear Hstep. erewrite <-(of_to_class e0) in Hred; [|eassumption].
         rewrite proj2_prog_union in H5;[|apply Hcan_link].
